make sure binary search example can be printed with string names as well as with Z names

bedrock2/src/Examples/BinarySearch.v
@@ -5,18 +5,23 @@ Require bedrock2.NotationsInConstr.
 Import BinInt String.
 Local Open Scope string_scope. Local Open Scope Z_scope. Local Open Scope list_scope.
 
+Class bsearch_names {p: unique! Syntax.parameters} := {
+  left : varname;
+  right : varname;
+  target : varname;
+  mid : varname;
+  tmp : varname;
+}.
+
 Section bsearch.
   Import bedrock2.NotationsInConstr.
-  Context {p : unique! StringNamesSyntax.parameters} {b : BasicALU.operations}.
+  Local Coercion var{p : unique! Syntax.parameters}(x : @varname p): @expr.expr p :=
+    @expr.var p x.
+
+  Context {p : unique! Syntax.parameters} {b : BasicALU.operations}.
   Local Coercion literal (z : Z) : expr := expr.literal z.
-  Local Coercion var (x : String.string) : expr := expr.var x.
 
-  Let left : varname := "left".
-  Let right : varname := "right".
-  Let target : varname := "target".
-
-  Let mid : varname := "mid".
-  Let tmp : varname := "tmp".
+  Context {names: unique! bsearch_names}.
 
   Definition bsearch := ((left::right::target::nil), (left::nil), bedrock_func_body:(
     while (left < right) {{
@@ -33,6 +38,56 @@ End bsearch.
 
 Require bedrock2.BasicC64Syntax.
 
+Local Instance bsearch_string_names:
+  @bsearch_names (StringNamesSyntax.make BasicC64Syntax.params) :=
+{
+  left := "left";
+  right := "right";
+  target := "target";
+  mid := "mid";
+  tmp := "tmp";
+}.
+
 Example bsearch_c_string := Eval compute in
   BasicC64Syntax.c_func "bsearch" (bsearch (b:=BasicC64Syntax.BasicALU)).
-(* Print bsearch_c_string. *)
+
+Print bsearch_c_string.
+
+Require bedrock2.ZNamesSyntax.
+
+Local Instance bsearch_string_ZNames:
+  @bsearch_names ZNamesSyntax.ZNames :=
+{
+  left := 1;
+  right := 2;
+  target := 3;
+  mid := 4;
+  tmp := 5;
+}.
+
+Require Import bedrock2.Basic_bopnames.
+
+Class my_parameters := {
+  varname: Set;
+  funcname: Set;
+  actname: Set;
+}.
+
+Local Instance make (p: my_parameters) : Syntax.parameters := {|
+  Syntax.varname := @varname p;
+  Syntax.funname := @funcname p;
+  Syntax.actname := @actname p;
+  Syntax.bopname := Basic_bopnames.bopname;
+|}.
+
+Import bopname.
+
+Local Instance MyBasicALU{p: my_parameters}: BasicALU.operations :=
+  BasicALU.Build_operations _ add sub mul and or xor sru slu srs lts ltu eq.
+
+Example bsearch_z_ast{p: unique! my_parameters} :=
+  Eval cbv [bsearch left right target mid tmp ZNamesSyntax.ZNames bsearch_string_ZNames
+            var literal] in
+    @bsearch ZNamesSyntax.ZNames MyBasicALU bsearch_string_ZNames.
+
+Print bsearch_z_ast.
